thys/No_Least_Support_Counterexample.thy
@@ -1,0 +1,139 @@
+theory No_Least_Support_Counterexample
+  imports Generic_Barendregt_Enhanced_Rule_Induction "HOL-Library.Stream"
+    "Infinitary_Lambda_Calculus.Embed_var_ivar"
+begin
+
+locale Nominal = Small dummy
+for dummy :: 'A
++
+fixes (* 'T: term-like entities *)
+Tmap :: "('A \<Rightarrow> 'A) \<Rightarrow> 'T \<Rightarrow> 'T"
+assumes  
+Tmap_id: "Tmap id = id"
+and
+Tmap_comp: "\<And>\<sigma> \<tau>. ssbij \<sigma> \<Longrightarrow> ssbij \<tau> \<Longrightarrow> Tmap (\<sigma> o \<tau>) = Tmap \<sigma> o Tmap \<tau>"
+and
+small_support: "\<And>t. \<exists>A. small A \<and> (\<forall>\<sigma>. ssbij \<sigma> \<longrightarrow> (\<forall>a\<in>A. \<sigma> a = a) \<longrightarrow> Tmap \<sigma> t = t)"
+begin
+
+definition supports where
+  "supports A t = (\<forall>\<sigma>. ssbij \<sigma> \<longrightarrow> (\<forall>a\<in>A. \<sigma> a = a) \<longrightarrow> Tmap \<sigma> t = t)"
+
+lemma small_Diff: "small A \<Longrightarrow> small (A - B)"
+  by (meson Diff_subset card_of_subset_bound small_def)
+lemma small_Int: "small A \<Longrightarrow> small (A \<inter> B)"
+  by (metis Diff_Diff_Int small_Diff)
+
+end
+
+definition "eq_ae s t = finite {i. snth s i \<noteq> snth t i}"
+
+lemma eq_ae_suffix: "eq_ae s t = (\<exists>i. sdrop i s = sdrop i t)"
+  unfolding eq_ae_def
+proof (safe, goal_cases)
+  case 1
+  then show ?case
+    apply (intro exI[of _ "Max (insert 0 (Suc ` {i. s !! i \<noteq> t !! i}))"])
+    apply (auto simp: Max.insert_remove smap_alt[of id, simplified stream.map_id id_apply]
+      mono_Max_commute[symmetric, of Suc, simplified mono_def, simplified] sdrop_snth
+      simp flip: snth.simps)
+    apply (smt (verit) Collect_empty_eq Max_less_iff add.commute less_add_Suc2 mem_Collect_eq verit_comp_simplify1(1))
+    done
+next
+  case (2 i)
+  then show ?case
+    by (safe intro!: finite_subset[of _ "{0 ..< i}", simplified])
+      (metis add_diff_inverse_nat atLeast0LessThan lessThan_iff sdrop_snth)
+qed
+
+lemma eq_ae_refl: "eq_ae s s"
+  by (auto simp: eq_ae_def)
+
+lemma eq_ae_sym: "eq_ae s t \<Longrightarrow> eq_ae t s"
+  by (auto simp: eq_ae_def elim: finite_subset[rotated])
+
+lemma eq_ae_trans: "eq_ae s t \<Longrightarrow> eq_ae t u \<Longrightarrow> eq_ae s u"
+  unfolding eq_ae_suffix
+  apply (elim exE)
+  subgoal for i j
+    apply (rule exI[of _ "max i j"])
+    apply (metis add.commute max.commute nat_minus_add_max sdrop_add)
+    done
+  done
+
+lemma eq_ae_equivp: "equivp eq_ae"
+  by (simp add: eq_ae_refl eq_ae_sym eq_ae_trans equivpI reflpI sympI transpI)
+
+quotient_type 'a item = "'a stream" / eq_ae
+  by (rule eq_ae_equivp)
+
+lift_definition map_item :: "('a \<Rightarrow> 'b) \<Rightarrow> 'a item \<Rightarrow> 'b item" is smap
+  unfolding eq_ae_suffix
+  apply (elim exE)
+  subgoal for f s t i
+    apply (rule exI[of _ i])
+    apply auto
+    done
+  done
+
+interpretation Small "undefined :: ivar"
+  by standard (simp_all add: regularCard_ivar infinite)
+
+interpretation Nominal "undefined :: ivar" map_item
+  apply standard
+  subgoal
+    by (rule ext, transfer) (auto simp: eq_ae_refl)
+  subgoal for \<sigma> \<tau>
+    by (rule ext, transfer) (auto simp: eq_ae_refl stream.map_comp)
+  subgoal for t
+    apply transfer
+    subgoal for s
+      apply (rule exI[of _ "sset s"])
+      apply safe
+      subgoal
+        unfolding small_def
+        using countable_card_ivar countable_sset by blast
+      subgoal
+        by (auto simp: eq_ae_refl stream.map_ident cong: stream.map_cong)
+      done
+    done
+  done
+
+lift_definition inats :: "ivar item" is "smap iVariable nats" .
+
+lemma small_from: "small (iVariable ` {n ..})"
+  unfolding small_def
+  by (rule countable_card_ivar) auto
+
+lemma supports_inats: "supports (iVariable ` {n ..}) inats"
+  unfolding supports_def
+  apply transfer
+  apply safe
+  subgoal for n \<sigma>
+    by (auto simp: stream.map_comp eq_ae_suffix intro!: exI[of _ n] stream.map_cong)
+  done
+
+context
+  assumes minimal: "\<exists>A. small A \<and> supports A t \<and> (\<forall>B. small B \<longrightarrow> supports B t \<longrightarrow> A \<subseteq> B)"
+begin
+
+lemma False
+proof -
+  from minimal obtain A where "small A" "supports A inats" "\<forall>B. small B \<longrightarrow> supports B inats \<longrightarrow> A \<subseteq> B"
+    by blast
+  then have *: "A \<subseteq> iVariable ` {n..}" for n
+    using small_from[of n] supports_inats[of n]
+    by auto
+  have "iVariable x \<notin> A" for x
+    using *[of "Suc x"] by auto
+  with small_ssbij[of "range iVariable" "range iVariable" A] small_from[of 0] \<open>small A\<close> obtain \<sigma> where
+    "ssbij \<sigma>" "\<sigma> ` range iVariable \<inter> range iVariable = {}" "\<forall>a\<in>A. \<sigma> a = a"
+    by auto
+  then show False
+    using \<open>supports A inats\<close>[unfolded supports_def, rule_format, where \<sigma> = \<sigma>]
+    by transfer (auto simp: stream.map_comp o_def eq_ae_suffix stream_eq_nth)
+qed
+
+end
+
+end
